lean4_port/NearLinear4ct.lean
@@ -1,6 +1,7 @@
 -- core value types & helpers
 import NearLinear4ct.OptIdx
 import NearLinear4ct.SmallNatPair
+import NearLinear4ct.Queue
 import NearLinear4ct.Util
 import NearLinear4ct.UtilProofs
 import NearLinear4ct.Mapping
